theories/rules.v
@@ -2,25 +2,18 @@ From cap_machine Require Export lang.
 From iris.base_logic Require Export invariants gen_heap.
 From iris.program_logic Require Export weakestpre lifting.
 From iris.proofmode Require Import tactics.
-From iris.algebra Require Import frac auth gmap agree.
+From iris.algebra Require Import frac.
 
 (* CMRΑ for memory *)
 Class memG Σ := MemG {
   mem_invG : invG Σ;
-  mem_gen_memG :> gen_heapG Addr Word Σ;
-}.
+  mem_gen_memG :> gen_heapG Addr Word Σ; }.
+
 (* CMRA for registers *)
 Class regG Σ := RegG {
   reg_invG : invG Σ;
-  reg_gen_regG :> gen_heapG RegName Word Σ; (* TODO: change this to agreement  *)
-(*                                              instead of exclusive agreement *)
-                  }.
+  reg_gen_regG :> gen_heapG RegName Word Σ; }.
 
-(* Class regG Σ := RegG { *)
-(*    reg_invG : invG Σ; *)
-(*    reg_gen_regG :> gen_regG RegName Word Σ }. *)
-
-  
 
 (* invariants for memory, and a state interpretation for (mem,reg) *)
 Instance memG_irisG `{memG Σ, regG Σ} : irisG cap_lang Σ := {
@@ -39,22 +32,14 @@ Notation "a ↦ₐ { q } w" := (mapsto (L:=Addr) (V:=Word) a q w)
   (at level 20, q at level 50, format "a  ↦ₐ { q }  w") : bi_scope.
 Notation "a ↦ₐ w" := (mapsto (L:=Addr) (V:=Word) a 1 w) (at level 20) : bi_scope.
 
-Lemma heap_mapsto_notduplicable `{memG Σ} a w :
-  (a ↦ₐ w ∗ a ↦ₐ w → False)%I. 
-Proof.
-  iIntros "[Ha1 Ha2]".
-  iCombine "Ha1 Ha2" as "Ha".
-  iDestruct (mapsto_valid with "Ha") as %Hf. contradiction.  
-Qed.
-
 (* temporary and permanent invariants *)
-Inductive inv_kind := T | F. 
+Inductive inv_kind := T | P. 
 Definition logN : namespace := nroot .@ "logN".
 
-Definition inv_cap `{memG Σ, regG Σ, inG Σ fracR} (t : inv_kind) P (ι : namespace) (γ : gname) :=
+Definition inv_cap `{memG Σ, regG Σ, inG Σ fracR} (t : inv_kind) iP (ι : namespace) (γ : gname) :=
   match t with
-  | T => inv ι (P ∨ (own γ 1%Qp))%I
-  | F => inv ι P
+  | T => inv ι (iP ∨ (own γ 1%Qp))%I
+  | P => inv ι iP
   end. 
 
 Section cap_lang_rules.
@@ -236,13 +221,14 @@ Section cap_lang_rules.
  (* --------------------------------------------------------------------------------- *)
  (* -------------------------------- SUCCESS RULES ---------------------------------- *)
    
-   Lemma wp_load_success r1 r2 pc_p pc_g pc_b pc_e pc_a w w' w'' p g b e a φ :
+   Lemma wp_load_success r1 r2 pc_p pc_g pc_b pc_e pc_a w w' w'' p g b e a pc_a' φ :
     cap_lang.decode w = Load r1 r2 →
     isCorrectPC (inr ((pc_p,pc_g),pc_b,pc_e,pc_a)) →
     readAllowed p = true ∧ withinBounds ((p, g), b, e, a) = true →
+    (pc_a + 1)%a = Some pc_a' →
     r1 ≠ PC →
     
-    ▷ ( PC ↦ᵣ inr ((pc_p,pc_g),pc_b,pc_e,(pc_a + 1)%Z) ∗ r1 ↦ᵣ w' -∗
+    ▷ ( PC ↦ᵣ inr ((pc_p,pc_g),pc_b,pc_e,pc_a') ∗ r1 ↦ᵣ w' -∗
       WP Executable {{ φ }} )
     ∗ PC ↦ᵣ inr ((pc_p,pc_g),pc_b,pc_e,pc_a)
     ∗ pc_a ↦ₐ w
@@ -252,7 +238,7 @@ Section cap_lang_rules.
     ⊢
     WP Executable {{ φ }}.
    Proof.
-     intros Hinstr Hvpc [Hra Hwb] Hne1. 
+     intros Hinstr Hvpc [Hra Hwb] Hpca' Hne1. 
      iIntros "(Hφ & Hpc & Hi & Hr1 & Hr2 & Hr2a)".
      iApply wp_lift_step_fupd; eauto.
      iIntros (σ1 l1 l2 n) "Hσ1 /=". destruct σ1; simpl.
@@ -276,7 +262,7 @@ Section cap_lang_rules.
                               (Executable,_));
          eauto; simpl; try congruence. 
         rewrite /withinBounds in Hwb; rewrite Hr2 Hra Hwb /updatePC /= Hpc_new1.
-          by rewrite /update_reg /= Ha.
+        by rewrite Hpca' /update_reg /= Ha.
      - iMod (fupd_intro_mask' ⊤) as "H"; eauto.
        iModIntro. 
        iIntros (e1 σ2 efs Hstep).
@@ -333,15 +319,17 @@ Section cap_lang_rules.
    Qed.
    
 
-   Lemma wp_subseg_success pc_p pc_g pc_b pc_e pc_a w dst r1 r2 p g b e a n1 n2 φ :
+   Lemma wp_subseg_success pc_p pc_g pc_b pc_e pc_a pc_a' w dst r1 r2 p g b e a n1 n2 a1 a2 φ :
      cap_lang.decode w = Subseg dst (inr r1) (inr r2) →
      isCorrectPC (inr ((pc_p,pc_g),pc_b,pc_e,pc_a)) →
+     (pc_a + 1)%a = Some pc_a' →
+     z_to_addr n1 = Some a1 ∧ z_to_addr n2 = Some a2 →
      p ≠ E →
      dst ≠ PC →
-     isWithin n1 n2 b e = true →
+     isWithin a1 a2 b e = true →
      
-     ▷ ( PC ↦ᵣ inr ((pc_p,pc_g),pc_b,pc_e,(pc_a + 1)%Z)
-            ∗ dst ↦ᵣ inr (p, g, n1, if (n2 =? -42)%Z then None else Some n2, a)
+     ▷ ( PC ↦ᵣ inr ((pc_p,pc_g),pc_b,pc_e,pc_a')
+            ∗ dst ↦ᵣ inr (p, g, a1, if (a2 =? -42)%a then None else Some a2, a)
             -∗  WP Executable {{ φ }} )
        ∗ PC ↦ᵣ inr ((pc_p,pc_g),pc_b,pc_e,pc_a)
        ∗ pc_a ↦ₐ w
@@ -351,7 +339,7 @@ Section cap_lang_rules.
        ⊢
        WP Executable {{ φ }}.
    Proof.
-     intros Hinstr Hvpc Hpne Hdstne Hwb.
+     intros Hinstr Hvpc Hpca' [Hn1 Hn2] Hpne Hdstne Hwb.
      iIntros "(Hφ & HPC & Hpc_a & Hdst & Hr1 & Hr2)".
      iApply wp_lift_step_fupd; eauto.
      iIntros (σ1 l1 l2 n) "Hσ1 /=". destruct σ1; simpl.
@@ -362,8 +350,8 @@ Section cap_lang_rules.
      iDestruct (@gen_heap_valid with "Hr Hr1") as %?.
      iDestruct (@gen_heap_valid with "Hr Hr2") as %?.
      option_locate_mr m r.
-     assert (<[dst:=inr (p, g, n1, if (n2 =? -42)%Z then None
-                                   else Some n2, a)]>
+     assert (<[dst:=inr (p, g, a1, if (a2 =? -42)%a then None
+                                   else Some a2, a)]>
              r !r! PC = (inr (pc_p, pc_g, pc_b, pc_e, pc_a)))
        as Hpc_new1.
      { rewrite (locate_ne_reg _ _ _ (inr (pc_p, pc_g, pc_b, pc_e, pc_a))); eauto. }
@@ -371,36 +359,38 @@ Section cap_lang_rules.
      iSplit.
      - rewrite /reducible.
        iExists [],Executable,
-       (updatePC (update_reg (r,m) dst (inr ((p, g), n1,
-            if Z.eqb n2 (-42)%Z then None else Some n2, a)))).2,[].
+       (updatePC (update_reg (r,m) dst (inr ((p, g), a1,
+            if (a2 =? (-42))%a then None else Some a2, a)))).2,[].
        iPureIntro.
        constructor.
        apply (step_exec_instr (r,m) pc_p pc_g pc_b pc_e pc_a
                               (Subseg dst (inr r1) (inr r2))
                               (Executable,_)); eauto; simpl; try congruence.
        rewrite Hdst. destruct p; (try congruence;
-       by rewrite Hr1 Hr2 Hwb /updatePC /update_reg /= Hpc_new1).
+        by rewrite Hr1 Hr2 Hn1 Hn2 Hwb /updatePC /update_reg /= Hpc_new1 Hpca').
      - destruct p; try congruence;
         (iMod (fupd_intro_mask' ⊤) as "H"; eauto;
          iModIntro;
          iIntros (e1 σ2 efs Hstep);
          inv_head_step_advanced m r HPC Hpc_a Hinstr Hstep Hpc_new1;
-         rewrite Hdst Hr1 Hr2 Hwb /updatePC /update_reg Hpc_new1 /=;
+         rewrite Hdst Hr1 Hr2 Hn1 Hn2 Hwb /updatePC /update_reg Hpc_new1 Hpca' /=;
          inv_head_step;
-         rewrite Hdst Hr1 Hr2 Hwb /updatePC /update_reg Hpc_new1 /= in Hstep;
+         rewrite Hdst Hr1 Hr2 Hn1 Hn2 Hwb /updatePC /update_reg Hpc_new1 Hpca' /= in Hstep;
          iMod (@gen_heap_update with "Hr Hdst") as "[Hr Hdst]";
          iMod (@gen_heap_update with "Hr HPC") as "[$ HPC]";
          iSpecialize ("Hφ" with "[HPC Hdst]"); iFrame;
          iModIntro; iNext; iFrame).
    Qed.
 
-   Lemma wp_subseg_success_pc pc_p pc_g pc_b pc_e pc_a w r1 r2 n1 n2 φ :
+   Lemma wp_subseg_success_pc pc_p pc_g pc_b pc_e pc_a pc_a' w r1 r2 n1 n2 a1 a2 φ :
      cap_lang.decode w = Subseg PC (inr r1) (inr r2) →
      isCorrectPC (inr ((pc_p,pc_g),pc_b,pc_e,pc_a)) →
+     (pc_a + 1)%a = Some pc_a' →
+     z_to_addr n1 = Some a1 ∧ z_to_addr n2 = Some a2 →
      pc_p ≠ E →
-     isWithin n1 n2 pc_b pc_e = true →
+     isWithin a1 a2 pc_b pc_e = true →
      
-     ▷ ( PC ↦ᵣ inr ((pc_p,pc_g),n1,if (n2 =? -42)%Z then None else Some n2,(pc_a + 1)%Z)
+     ▷ ( PC ↦ᵣ inr ((pc_p,pc_g),a1,if (a2 =? -42)%a then None else Some a2,pc_a')
             -∗  WP Executable {{ φ }} )
        ∗ PC ↦ᵣ inr ((pc_p,pc_g),pc_b,pc_e,pc_a)
        ∗ pc_a ↦ₐ w
@@ -409,7 +399,7 @@ Section cap_lang_rules.
        ⊢
        WP Executable {{ φ }}.
    Proof.
-     intros Hinstr Hvpc Hpne Hwb.
+     intros Hinstr Hvpc Hpca' [Hn1 Hn2] Hpne Hwb.
      iIntros "(Hφ & HPC & Hpc_a & Hr1 & Hr2)".
      iApply wp_lift_step_fupd; eauto.
      iIntros (σ1 l1 l2 n) "Hσ1 /=". destruct σ1; simpl.
@@ -419,44 +409,45 @@ Section cap_lang_rules.
      iDestruct (@gen_heap_valid with "Hr HPC") as %?.
      iDestruct (@gen_heap_valid with "Hr Hr2") as %?.
      option_locate_mr m r.
-     assert (<[PC:=inr (pc_p, pc_g, n1, if (n2 =? -42)%Z then None
-                                   else Some n2, pc_a)]>
-             r !r! PC = inr (pc_p, pc_g, n1, if (n2 =? -42)%Z then None
-                                   else Some n2, pc_a))
+     assert (<[PC:=inr (pc_p, pc_g, a1, if (a2 =? -42)%a then None
+                                   else Some a2, pc_a)]>
+             r !r! PC = inr (pc_p, pc_g, a1, if (a2 =? -42)%a then None
+                                   else Some a2, pc_a))
        as Hpc_new1; first by rewrite /RegLocate lookup_insert. 
      iApply fupd_frame_l. 
      iSplit.
      - rewrite /reducible.
        iExists [],Executable,
-       (updatePC (update_reg (r,m) PC (inr ((pc_p, pc_g), n1,
-            if Z.eqb n2 (-42)%Z then None else Some n2, pc_a)))).2,[].
+       (updatePC (update_reg (r,m) PC (inr ((pc_p, pc_g), a1,
+            if (a2 =? (-42))%a then None else Some a2, pc_a)))).2,[].
        iPureIntro.
        constructor.
        apply (step_exec_instr (r,m) pc_p pc_g pc_b pc_e pc_a
                               (Subseg PC (inr r1) (inr r2))
                               (Executable,_)); eauto; simpl; try congruence.
        rewrite HPC. destruct pc_p; (try congruence;
-       by rewrite Hr1 Hr2 Hwb /updatePC /update_reg /= Hpc_new1).
+       by rewrite Hr1 Hr2 Hn1 Hn2 Hwb /updatePC /update_reg /= Hpc_new1 Hpca').
      - destruct pc_p; try congruence;
         (iMod (fupd_intro_mask' ⊤) as "H"; eauto;
          iModIntro;
          iIntros (e1 σ2 efs Hstep);
          inv_head_step_advanced m r HPC Hpc_a Hinstr Hstep Hpc_new1;
-         rewrite HPC Hr1 Hr2 Hwb /updatePC /update_reg Hpc_new1 /= insert_insert;
+         rewrite HPC Hr1 Hr2 Hn1 Hn2 Hwb /updatePC /update_reg Hpc_new1 Hpca' /= insert_insert;
          inv_head_step;
-         rewrite HPC Hr1 Hr2 Hwb /updatePC /update_reg Hpc_new1 /= insert_insert
+         rewrite HPC Hr1 Hr2 Hn1 Hn2 Hwb /updatePC /update_reg Hpc_new1 Hpca' /= insert_insert
            in Hstep;
          iMod (@gen_heap_update with "Hr HPC") as "[$ HPC]";
          iSpecialize ("Hφ" with "[HPC]"); iFrame;
          iModIntro; iNext; iFrame).
    Qed.
 
-   Lemma wp_IsPtr_success_S pc_p pc_g pc_b pc_e pc_a w dst r ptr w' φ :
+   Lemma wp_IsPtr_success_S pc_p pc_g pc_b pc_e pc_a pc_a' w dst r ptr w' φ :
      cap_lang.decode w = IsPtr dst r →
      isCorrectPC (inr ((pc_p,pc_g),pc_b,pc_e,pc_a)) →
+     (pc_a + 1)%a = Some pc_a' →
      dst ≠ PC →  
 
-      ▷ ( PC ↦ᵣ inr ((pc_p,pc_g),pc_b,pc_e,(pc_a+1)%Z) ∗ dst ↦ᵣ inl 1%Z
+      ▷ ( PC ↦ᵣ inr ((pc_p,pc_g),pc_b,pc_e,pc_a') ∗ dst ↦ᵣ inl 1%Z
             -∗  WP Executable {{ φ }} )
        ∗ PC ↦ᵣ inr ((pc_p,pc_g),pc_b,pc_e,pc_a)
        ∗ pc_a ↦ₐ w
@@ -465,7 +456,7 @@ Section cap_lang_rules.
        ⊢
        WP Executable {{ φ }}.
    Proof.
-     intros Hinstr Hvpc Hne.
+     intros Hinstr Hvpc Hpca' Hne.
      iIntros "(Hφ & HPC & Hpc_a & Hr & Hdst)".
      iApply wp_lift_step_fupd; eauto.
      iIntros (σ1 l1 l2 n) "Hσ1 /=". destruct σ1; simpl.
@@ -480,30 +471,31 @@ Section cap_lang_rules.
      iApply fupd_frame_l. 
      iSplit.
      - rewrite /reducible.
-       iExists [], Executable,(<[PC:=inr (pc_p, pc_g, pc_b, pc_e, (pc_a + 1)%Z)]> (<[dst:=inl 1%Z]> r0), m), [].
+       iExists [], Executable,(<[PC:=inr (pc_p, pc_g, pc_b, pc_e, pc_a')]> (<[dst:=inl 1%Z]> r0), m), [].
        iPureIntro.
        constructor. 
        apply (step_exec_instr (r0,m) pc_p pc_g pc_b pc_e pc_a
                               (IsPtr dst r)
                               (Executable,_)); eauto; simpl; try congruence.
-         by rewrite Hr /update_reg /updatePC /= Hpc_new1 /update_reg /updatePC /=.
+         by rewrite Hr /update_reg /updatePC /= Hpc_new1 Hpca' /update_reg /updatePC /=.
      - iMod (fupd_intro_mask' ⊤) as "H"; eauto.
        iModIntro.
        iIntros (e1 σ2 efs Hstep).
        inv_head_step_advanced m r0 HPC Hpc_a Hinstr Hstep Hpc_new1.
-       rewrite Hr /updatePC /update_reg /= Hpc_new1 /=.
+       rewrite Hr /updatePC /update_reg /= Hpc_new1 Hpca' /=.
        iMod (@gen_heap_update with "Hr0 Hdst") as "[Hr0 Hdst]".
        iMod (@gen_heap_update with "Hr0 HPC") as "[$ HPC]".
        iSpecialize ("Hφ" with "[HPC Hdst]"); iFrame.
        iModIntro. iNext. iFrame.
    Qed.
 
-   Lemma wp_IsPtr_success_F pc_p pc_g pc_b pc_e pc_a w dst r z w' φ :
+   Lemma wp_IsPtr_success_F pc_p pc_g pc_b pc_e pc_a pc_a' w dst r z w' φ :
      cap_lang.decode w = IsPtr dst r →
      isCorrectPC (inr ((pc_p,pc_g),pc_b,pc_e,pc_a)) →
+     (pc_a + 1)%a = Some pc_a' →
      dst ≠ PC →  
 
-      ▷ ( PC ↦ᵣ inr ((pc_p,pc_g),pc_b,pc_e,(pc_a+1)%Z) ∗ dst ↦ᵣ inl 0%Z
+      ▷ ( PC ↦ᵣ inr ((pc_p,pc_g),pc_b,pc_e,pc_a') ∗ dst ↦ᵣ inl 0%Z
             -∗  WP Executable {{ φ }} )
        ∗ PC ↦ᵣ inr ((pc_p,pc_g),pc_b,pc_e,pc_a)
        ∗ pc_a ↦ₐ w
@@ -512,7 +504,7 @@ Section cap_lang_rules.
        ⊢
        WP Executable {{ φ }}.
    Proof.
-     intros Hinstr Hvpc Hne.
+     intros Hinstr Hvpc Hpca' Hne.
      iIntros "(Hφ & HPC & Hpc_a & Hr & Hdst)".
      iApply wp_lift_step_fupd; eauto.
      iIntros (σ1 l1 l2 n) "Hσ1 /=". destruct σ1; simpl.
@@ -527,18 +519,18 @@ Section cap_lang_rules.
      iApply fupd_frame_l. 
      iSplit.
      - rewrite /reducible.
-       iExists [], Executable,(<[PC:=inr (pc_p, pc_g, pc_b, pc_e, (pc_a + 1)%Z)]> (<[dst:=inl 0%Z]> r0), m), [].
+       iExists [], Executable,(<[PC:=inr (pc_p, pc_g, pc_b, pc_e, pc_a')]> (<[dst:=inl 0%Z]> r0), m), [].
        iPureIntro.
        constructor. 
        apply (step_exec_instr (r0,m) pc_p pc_g pc_b pc_e pc_a
                               (IsPtr dst r)
                               (Executable,_)); eauto; simpl; try congruence.
-       by rewrite Hr /update_reg /updatePC /= Hpc_new1 /update_reg /updatePC /=.
+       by rewrite Hr /update_reg /updatePC /= Hpc_new1 Hpca' /update_reg /updatePC /=.
      - iMod (fupd_intro_mask' ⊤) as "H"; eauto.
        iModIntro.
        iIntros (e1 σ2 efs Hstep).
        inv_head_step_advanced m r0 HPC Hpc_a Hinstr Hstep Hpc_new1.
-       rewrite Hr /updatePC /update_reg /= Hpc_new1 /=.
+       rewrite Hr /updatePC /update_reg /= Hpc_new1 Hpca' /=.
        iMod (@gen_heap_update with "Hr0 Hdst") as "[Hr0 Hdst]".
        iMod (@gen_heap_update with "Hr0 HPC") as "[$ HPC]".
        iSpecialize ("Hφ" with "[HPC Hdst]"); iFrame.
@@ -546,15 +538,16 @@ Section cap_lang_rules.
    Qed.
 
 
-   Lemma wp_store_success_local pc_p pc_g pc_b pc_e pc_a w dst src w'
+   Lemma wp_store_success_local pc_p pc_g pc_b pc_e pc_a pc_a' w dst src w'
          p g b e a p' g' b' e' a' φ :
      cap_lang.decode w = Store dst (inr src) →
      isCorrectPC (inr ((pc_p,pc_g),pc_b,pc_e,pc_a)) →
+     (pc_a + 1)%a = Some pc_a' →
      writeAllowed p = true ∧ withinBounds ((p, g), b, e, a) = true →
      isLocal g' = true ∧ (p = RWLX ∨ p = RWL) → 
      dst ≠ PC →
 
-     ▷ ( PC ↦ᵣ inr ((pc_p,pc_g),pc_b,pc_e,(pc_a+1)%Z) ∗ a ↦ₐ inr ((p',g'),b',e',a') 
+     ▷ ( PC ↦ᵣ inr ((pc_p,pc_g),pc_b,pc_e,pc_a') ∗ a ↦ₐ inr ((p',g'),b',e',a') 
             -∗  WP Executable {{ φ }} )
        ∗ PC ↦ᵣ inr ((pc_p,pc_g),pc_b,pc_e,pc_a)
        ∗ pc_a ↦ₐ w
@@ -564,7 +557,7 @@ Section cap_lang_rules.
        ⊢
        WP Executable {{ φ }}.
    Proof.
-     intros Hinstr Hvpc [Hwa Hwb] [Hlocal Hp] Hne; simpl in *. 
+     intros Hinstr Hvpc Hpca' [Hwa Hwb] [Hlocal Hp] Hne; simpl in *. 
      iIntros "(Hφ & HPC & Hpc_a & Hsrc & Hdst & Ha)".
      iApply wp_lift_step_fupd; eauto.
      iIntros (σ1 l1 l2 n) "Hσ1 /=". destruct σ1; simpl.
@@ -586,36 +579,18 @@ Section cap_lang_rules.
                               (Executable,_)); eauto; simpl; try congruence.
        rewrite Hdst Hwa Hwb /= Hsrc Hlocal.
        destruct Hp as [Hp | Hp]; try contradiction;
-         by rewrite Hp /updatePC /update_mem /= HPC.
+         by rewrite Hp /updatePC /update_mem /= HPC Hpca'.
      - iMod (fupd_intro_mask' ⊤) as "H"; eauto.
        iModIntro.
        iIntros (e1 σ2 efs Hstep).
        inv_head_step_advanced m r HPC Hpc_a Hinstr Hstep HPC.
        rewrite Hdst Hwa Hwb /= Hsrc Hlocal.
        destruct Hp as [Hp | Hp]; try contradiction;
-       ( rewrite Hp /updatePC /update_mem /= HPC /update_reg /=;
+       ( rewrite Hp /updatePC /update_mem /= HPC /update_reg /= Hpca';
          iMod (@gen_heap_update with "Hm Ha") as "[$ Ha]";
          iMod (@gen_heap_update with "Hr HPC") as "[$ HPC]";
          iSpecialize ("Hφ" with "[HPC Ha]"); iFrame; eauto ). 
    Qed. 
-       
-         
-   (* Store dst (inr src) => *)
-   (*    match RegLocate (reg φ) dst with *)
-   (*    | inl n => (Failed, φ) *)
-   (*    | inr ((p, g), b, e, a) => *)
-   (*      if writeAllowed p && withinBounds ((p, g), b, e, a) then *)
-   (*        match RegLocate (reg φ) src with *)
-   (*        | inl n => updatePC (update_mem φ a (RegLocate (reg φ) src)) *)
-   (*        | inr ((_, g'), _, _, _) => if isLocal g' then *)
-   (*                                     match p with *)
-   (*                                     | RWLX | RWL => updatePC (update_mem φ a (RegLocate (reg φ) src)) *)
-   (*                                     | _ => (Failed, φ) *)
-   (*                                     end *)
-   (*                                   else updatePC (update_mem φ a (RegLocate (reg φ) src)) *)
-   (*        end *)
-   (*      else (Failed, φ) *)
-   (*    end *)
        
        
  (* --------------------------------------------------------------------------------- *)
@@ -645,6 +620,39 @@ Section cap_lang_rules.
        constructor.
        apply (step_exec_instr (r,m) pc_p pc_g pc_b pc_e pc_a Halt
                               (Halted,_));
+         eauto; simpl; try congruence.
+     - iIntros (e2 σ2 efs Hstep).
+       inv_head_step_advanced m r HPC Hpc_a Hinstr Hstep HPC.
+       iFrame.
+       iModIntro. iNext. iModIntro. iSplitL; eauto. 
+       iApply "Hφ".
+       iFrame.
+   Qed.
+
+   Lemma wp_fail pc_p pc_g pc_b pc_e pc_a w :
+     cap_lang.decode w = Fail →
+     isCorrectPC (inr ((pc_p,pc_g),pc_b,pc_e,pc_a)) →
+     
+     {{{ PC ↦ᵣ inr ((pc_p,pc_g),pc_b,pc_e,pc_a) ∗ pc_a ↦ₐ w }}}
+       Executable 
+     {{{ RET FailedV; PC ↦ᵣ inr ((pc_p,pc_g),pc_b,pc_e,pc_a) ∗ pc_a ↦ₐ w }}}.
+   Proof.
+     intros Hinstr Hvpc. 
+     iIntros (φ) "[Hpc Hpca] Hφ".
+     iApply wp_lift_atomic_step_fupd; auto.
+     iIntros (σ1 l1 l2 n) "Hσ1 /=". destruct σ1; simpl.
+     iDestruct "Hσ1" as "[Hr Hm]".
+     iDestruct (@gen_heap_valid with "Hr Hpc") as %?.
+     iDestruct (@gen_heap_valid with "Hm Hpca") as %?.
+     option_locate_mr m r. 
+     iModIntro.
+     iSplitR.
+     - rewrite /reducible. 
+       iExists [],Failed,(r,m),[].       
+       iPureIntro.
+       constructor.
+       apply (step_exec_instr (r,m) pc_p pc_g pc_b pc_e pc_a Fail
+                              (Failed,_));
          eauto; simpl; try congruence.
      - iIntros (e2 σ2 efs Hstep).
        inv_head_step_advanced m r HPC Hpc_a Hinstr Hstep HPC.
